autoclrs/ch12-bst/CLRS.Ch12.BSTArray.TestMain.fst
@@ -1,13 +1,13 @@
-module CLRS.Ch12.BST.TestMain
+module CLRS.Ch12.BSTArray.TestMain
 #lang-pulse
 open Pulse.Lib.Pervasives
-open CLRS.Ch12.BST.ImplTest
+open CLRS.Ch12.BSTArray.ImplTest
 
 fn main ()
   requires emp
   returns r: bool
   ensures pure (r == true)
 {
-  let r = test_bst_ptr ();
+  let r = test_bstarray_search_insert ();
   r
 }
